`MLOAD` opcode equivalence (#12)
* Generate code for `MLOAD` opcode

* `MstoreSummary`: rename `mstore_activeWords` to `activeWords_comp`

* Add `Interfaces/MloadSummary.lean`

* `MstoreEquivalence`: `mstore_activeWords` -> `activeWords_comp`

* `EvmEquivalence.lean`: add comments to "K generated code" section

* `EvmEquivalence.lean`: add `Utils.ListByteArrayUtils`

* `EvmEquivalence.lean`: add `MLOAD` summary and equivalence

* `MstoreEquivalence.lean`: remove spurious `_Val*` in LHS

* `MstoreEquivalence`: `mstore_activeWords_eq` -> `activeWords_eq`

* Implement function `Bytes2Int` in `Prelude.lean`

* Update generated Lean code

* `EvmYulInterface`: add `fromByteArrayBigEndian_empty`

* `ListByteArrayUtils`: more `ByteArray` theorems

* `ListByteArrayUtils`: add `Axioms` section with `toList_eq` axiom

* `FuncInterface`: theorems for `Bytes2Int` `#range` `asWord` `chop`

* Add `Equivalence/MloadEquivalence.lean`

* Update generated code to latest version of `klean`

* `MloadSummary.lean`: remove spurious comment

EvmEquivalence/Equivalence/MstoreEquivalence.lean
@@ -14,7 +14,7 @@ namespace MstoreOpcodeEquivalence
 
 def mstoreLHS
   {GAS_CELL MEMORYUSED_CELL PC_CELL W0 W1 : SortInt}
-  {LOCALMEM_CELL _Val14 _Val15 _Val16 : SortBytes}
+  {LOCALMEM_CELL : SortBytes}
   {SCHEDULE_CELL : SortSchedule}
   {USEGAS_CELL : SortBool}
   {WS : SortWordStack}
@@ -206,14 +206,14 @@ theorem rw_mstoreLHS_mstoreRHS
   (defn_Val25 : «#memoryUsageUpdate» MEMORYUSED_CELL W0 32 = some _Val25)
   (req : _Val13 = true) :
   Rewrites
-  (@mstoreLHS GAS_CELL MEMORYUSED_CELL PC_CELL W0 W1 LOCALMEM_CELL _Val14 _Val15 _Val16 SCHEDULE_CELL USEGAS_CELL WS _DotVar0 _DotVar2 _Gen0 _Gen1 _Gen10 _Gen11 _Gen12 _Gen13 _Gen14 _Gen15 _Gen16 _Gen17 _Gen18 _Gen19 _Gen2 _Gen20 _Gen21 _Gen3 _Gen4 _Gen5 _Gen6 _Gen7 _Gen8 _Gen9 _K_CELL)
+  (@mstoreLHS GAS_CELL MEMORYUSED_CELL PC_CELL W0 W1 LOCALMEM_CELL SCHEDULE_CELL USEGAS_CELL WS _DotVar0 _DotVar2 _Gen0 _Gen1 _Gen10 _Gen11 _Gen12 _Gen13 _Gen14 _Gen15 _Gen16 _Gen17 _Gen18 _Gen19 _Gen2 _Gen20 _Gen21 _Gen3 _Gen4 _Gen5 _Gen6 _Gen7 _Gen8 _Gen9 _K_CELL)
   (@mstoreRHS _Val17 _Val24 _Val25 _Val16 SCHEDULE_CELL WS _DotVar0 _DotVar2 _Gen0 _Gen1 _Gen10 _Gen11 _Gen12 _Gen13 _Gen14 _Gen15 _Gen16 _Gen17 _Gen18 _Gen19 _Gen2 _Gen20 _Gen21 _Gen3 _Gen4 _Gen5 _Gen6 _Gen7 _Gen8 _Gen9 _K_CELL)
   := by apply (@Rewrites.MSTORE_SUMMARY_MSTORE_SUMMARY_USEGAS GAS_CELL MEMORYUSED_CELL PC_CELL W0 W1 _Val0 _Val1 _Val10 _Val17 _Val18 _Val19 _Val2 _Val20 _Val21 _Val22 _Val23 _Val24 _Val25 _Val3 _Val5 _Val6 _Val7 _Val8)
   <;> assumption
 
 theorem mstore_prestate_equiv
   {GAS_CELL MEMORYUSED_CELL PC_CELL W0 W1 : SortInt}
-  {LOCALMEM_CELL _Val14 _Val15 _Val16 : SortBytes}
+  {LOCALMEM_CELL : SortBytes}
   {SCHEDULE_CELL : SortSchedule}
   {USEGAS_CELL : SortBool}
   {WS : SortWordStack}
@@ -243,7 +243,7 @@ theorem mstore_prestate_equiv
   {_Gen9 : SortOutputCell}
   {_K_CELL : SortK}
   (symState : EVM.State) :
-  let lhs := (@mstoreLHS GAS_CELL MEMORYUSED_CELL PC_CELL W0 W1 LOCALMEM_CELL _Val14 _Val15 _Val16 SCHEDULE_CELL USEGAS_CELL WS _DotVar0 _DotVar2 _Gen0 _Gen1 _Gen10 _Gen11 _Gen12 _Gen13 _Gen14 _Gen15 _Gen16 _Gen17 _Gen18 _Gen19 _Gen2 _Gen20 _Gen21 _Gen3 _Gen4 _Gen5 _Gen6 _Gen7 _Gen8 _Gen9 _K_CELL)
+  let lhs := (@mstoreLHS GAS_CELL MEMORYUSED_CELL PC_CELL W0 W1 LOCALMEM_CELL SCHEDULE_CELL USEGAS_CELL WS _DotVar0 _DotVar2 _Gen0 _Gen1 _Gen10 _Gen11 _Gen12 _Gen13 _Gen14 _Gen15 _Gen16 _Gen17 _Gen18 _Gen19 _Gen2 _Gen20 _Gen21 _Gen3 _Gen4 _Gen5 _Gen6 _Gen7 _Gen8 _Gen9 _K_CELL)
   stateMap symState lhs =
   {symState with
     stack := (intMap W0) :: (intMap W1) :: wordStackMap WS
@@ -304,15 +304,15 @@ theorem mstore_poststate_equiv
     memory := memory_map rhs.memory
     } := by cases _Gen15; aesop (add simp [«_+Int_»])
 
-theorem mstore_activeWords_eq
+theorem activeWords_eq
   {MEMORYUSED_CELL W0 _Val25: SortInt}
   (defn_Val25 : «#memoryUsageUpdate» MEMORYUSED_CELL W0 32 = some _Val25)
   (W0ge0 : 0 ≤ W0)
   (W0small : W0 < UInt256.size)
   (mucge0 : 0 ≤ MEMORYUSED_CELL)
   (mucsmall : MEMORYUSED_CELL < UInt256.size) :
-  mstore_activeWords (intMap W0) (intMap MEMORYUSED_CELL) = intMap _Val25 := by
-  unfold mstore_activeWords
+  activeWords_comp (intMap W0) (intMap MEMORYUSED_CELL) = intMap _Val25 := by
+  unfold activeWords_comp
   rw [memoryUsageUpdate_rw, Option.some.injEq] at defn_Val25
   simp [←defn_Val25, intMap]; rw [UInt256.ofNat_toSigned]
   simp [UInt256.toSigned]; cases mucc: MEMORYUSED_CELL
@@ -465,7 +465,7 @@ theorem step_mstore_equiv
   -- It seems we need this hypothesis to achieve equivalence of behavior from the EVMYul side
   -- We keep the original `W0small` for convenience
   (W0small_realpolitik : W0 < UInt32.size) :
-  EVM.step_mstore (Int.toNat GAS_CELL) gasCost (stateMap symState (@mstoreLHS GAS_CELL MEMORYUSED_CELL PC_CELL W0 W1 LOCALMEM_CELL _Val14 _Val15 _Val16 SCHEDULE_CELL USEGAS_CELL WS _DotVar0 _DotVar2 _Gen0 _Gen1 _Gen10 _Gen11 _Gen12 _Gen13 _Gen14 _Gen15 _Gen16 _Gen17 _Gen18 _Gen19 _Gen2 _Gen20 _Gen21 _Gen3 _Gen4 _Gen5 _Gen6 _Gen7 _Gen8 _Gen9 _K_CELL)) =
+  EVM.step_mstore (Int.toNat GAS_CELL) gasCost (stateMap symState (@mstoreLHS GAS_CELL MEMORYUSED_CELL PC_CELL W0 W1 LOCALMEM_CELL SCHEDULE_CELL USEGAS_CELL WS _DotVar0 _DotVar2 _Gen0 _Gen1 _Gen10 _Gen11 _Gen12 _Gen13 _Gen14 _Gen15 _Gen16 _Gen17 _Gen18 _Gen19 _Gen2 _Gen20 _Gen21 _Gen3 _Gen4 _Gen5 _Gen6 _Gen7 _Gen8 _Gen9 _K_CELL)) =
   .ok (stateMap {symState with execLength := symState.execLength + 1} (@mstoreRHS _Val17 _Val24 _Val25 _Val16 SCHEDULE_CELL WS _DotVar0 _DotVar2 _Gen0 _Gen1 _Gen10 _Gen11 _Gen12 _Gen13 _Gen14 _Gen15 _Gen16 _Gen17 _Gen18 _Gen19 _Gen2 _Gen20 _Gen21 _Gen3 _Gen4 _Gen5 _Gen6 _Gen7 _Gen8 _Gen9 _K_CELL))
   := by
   cases cg: (Int.toNat GAS_CELL)
@@ -475,10 +475,10 @@ theorem step_mstore_equiv
   cases _Gen15; rw [mstore_prestate_equiv]; simp [mstoreLHS]
   rw [←EVM.step_mstore, EVM.step_mstore_summary] <;> first | assumption | try simp
   rw [mstore_poststate_equiv, mstoreRHS] <;> first | assumption | try simp
-  simp [mstore_activeWords, mstore_memory_write]
+  simp [activeWords_comp, mstore_memory_write]
   constructor; constructor <;> try constructor
   . sorry -- Gas goals are for now unproven
-  . rw [←mstore_activeWords, mstore_activeWords_eq defn_Val25] <;> assumption
+  . rw [←activeWords_comp, activeWords_eq defn_Val25] <;> assumption
   . rw [←mstore_memory_write, mstore_memory_write_eq defn_Val14 defn_Val15 defn_Val16]
     <;> assumption
   . rw [←UInt256.add_succ_mod_size, intMap_add_dist] <;> aesop
@@ -567,7 +567,7 @@ theorem X_mstore_equiv
   -- We keep the original `W0small` for convenience
   (W0small_realpolitik : W0 < UInt32.size) :
   EVM.X (UInt256.toNat (intMap GAS_CELL)) symValidJumps
-  (stateMap symState (@mstoreLHS GAS_CELL MEMORYUSED_CELL PC_CELL W0 W1 LOCALMEM_CELL _Val14 _Val15 _Val16 SCHEDULE_CELL USEGAS_CELL WS _DotVar0 _DotVar2 _Gen0 _Gen1 _Gen10 _Gen11 _Gen12 _Gen13 _Gen14 _Gen15 _Gen16 _Gen17 _Gen18 _Gen19 _Gen2 _Gen20 _Gen21 _Gen3 _Gen4 _Gen5 _Gen6 _Gen7 _Gen8 _Gen9 _K_CELL)) =
+  (stateMap symState (@mstoreLHS GAS_CELL MEMORYUSED_CELL PC_CELL W0 W1 LOCALMEM_CELL SCHEDULE_CELL USEGAS_CELL WS _DotVar0 _DotVar2 _Gen0 _Gen1 _Gen10 _Gen11 _Gen12 _Gen13 _Gen14 _Gen15 _Gen16 _Gen17 _Gen18 _Gen19 _Gen2 _Gen20 _Gen21 _Gen3 _Gen4 _Gen5 _Gen6 _Gen7 _Gen8 _Gen9 _K_CELL)) =
   .ok (.success (stateMap {symState with execLength := symState.execLength + 2} (@mstoreRHS _Val17 _Val24 _Val25 _Val16 SCHEDULE_CELL WS _DotVar0 _DotVar2 _Gen0 _Gen1 _Gen10 _Gen11 _Gen12 _Gen13 _Gen14 _Gen15 _Gen16 _Gen17 _Gen18 _Gen19 _Gen2 _Gen20 _Gen21 _Gen3 _Gen4 _Gen5 _Gen6 _Gen7 _Gen8 ⟨.empty⟩ _K_CELL)) .empty)
   := by
   cases cg: (Int.toNat GAS_CELL)
@@ -585,7 +585,7 @@ theorem X_mstore_equiv
       simp [memoryExpansionCost_mstore _ (intMap W0) (intMap MEMORYUSED_CELL)]
       simp [EVM.Cₘ]
       sorry
-    . rw [mstore_activeWords_eq defn_Val25] <;> assumption
+    . rw [activeWords_eq defn_Val25] <;> assumption
     . rw [mstore_memory_write_eq defn_Val14 defn_Val15 defn_Val16] <;> assumption
     . aesop
   . -- Enough Gas
