EvmEquivalence/Summaries/MloadSummary.lean
@@ -1,0 +1,180 @@
+import EvmYul.EVM.Semantics
+import EvmYul.EVM.GasConstants
+import EvmEquivalence.Interfaces.EvmYulInterface
+import EvmEquivalence.Summaries.MstoreSummary
+
+open EvmYul
+open EVM
+open EvmYul.State
+
+namespace MloadSummary
+
+section
+
+variable (gas gasCost : ℕ)
+variable (symStack : Stack UInt256)
+variable (symPc symGasAvailable symRefund offset : UInt256)
+variable (symActiveWords : UInt256)
+variable (symExecLength : ℕ)
+variable (symReturnData symCode symMemory : ByteArray)
+variable (symAccessedStorageKeys : Batteries.RBSet (AccountAddress × UInt256) Substate.storageKeysCmp)
+variable (symAccounts : AccountMap)
+variable (symCodeOwner : AccountAddress)
+variable (symPerm : Bool)
+
+variable (symValidJumps : Array UInt256)
+
+@[simp]
+abbrev mloadEVM := @Operation.MLOAD .EVM
+
+@[simp]
+abbrev mload_instr : Option (Operation .EVM × Option (UInt256 × Nat)) :=
+  some ⟨mloadEVM, none⟩
+
+@[simp]
+abbrev EVM.step_mload : Transformer :=
+  EVM.step gas gasCost mload_instr
+
+@[simp]
+abbrev EvmYul.step_mload : Transformer :=
+  EvmYul.step mloadEVM
+
+abbrev activeWords_comp := MstoreSummary.activeWords_comp
+
+theorem EvmYul.step_mload_summary (symState : EVM.State):
+  let ss := {symState with
+    stack := offset :: symStack,
+    pc := symPc
+    gasAvailable := symGasAvailable,
+    executionEnv := {symState.executionEnv with
+                  code := symCode,
+                  codeOwner := symCodeOwner
+                  perm := symPerm},
+    accountMap := symAccounts,
+    activeWords := symActiveWords,
+    memory := symMemory,
+    substate := {symState.substate with
+                 accessedStorageKeys :=  symAccessedStorageKeys
+                 refundBalance := symRefund}
+    returnData := symReturnData,
+    execLength := symExecLength}
+  EvmYul.step_mload ss =
+  .ok {ss with
+    stack := (EvmYul.MachineState.lookupMemory ss.toMachineState offset) :: symStack,
+    pc := symPc + .ofNat 1,
+    activeWords := activeWords_comp offset symActiveWords} := by aesop
+
+theorem EVM.step_mload_summary (gas_pos : 0 < gas) (symState : EVM.State):
+  let ss := {symState with
+    stack := offset :: symStack,
+    pc := symPc
+    gasAvailable := symGasAvailable,
+    executionEnv := {symState.executionEnv with
+                  code := symCode,
+                  codeOwner := symCodeOwner
+                  perm := symPerm},
+    accountMap := symAccounts,
+    activeWords := symActiveWords,
+    memory := symMemory,
+    substate := {symState.substate with
+                 accessedStorageKeys :=  symAccessedStorageKeys
+                 refundBalance := symRefund}
+    returnData := symReturnData,
+    execLength := symExecLength}
+  EVM.step_mload gas gasCost ss =
+    .ok {ss with
+          stack := (EvmYul.MachineState.lookupMemory ss.toMachineState offset) :: symStack
+          pc := symPc + (.ofNat 1),
+          gasAvailable := symGasAvailable - UInt256.ofNat gasCost,
+          activeWords := activeWords_comp offset symActiveWords
+          execLength := symExecLength + 1} := by
+  cases gas; contradiction
+  simp [step_mload, EVM.step]
+  have := EvmYul.step_mload_summary symStack symPc (symGasAvailable - UInt256.ofNat gasCost) symRefund offset symActiveWords (symExecLength + 1) symReturnData symCode symMemory
+  simp [EvmYul.step_mload, Operation.MLOAD] at this; aesop
+
+@[simp]
+theorem decode_singleton_mload :
+  decode ⟨#[0x51]⟩ (.ofNat 0) = some ⟨mloadEVM, none⟩ := rfl
+
+@[simp]
+def value_and_activeWords_gas (s : EVM.State) :=
+  UInt256.ofNat (MachineState.M symActiveWords.toNat s.stack[0]!.toNat 32)
+
+@[simp]
+theorem memoryExpansionCost_mload (symState : EVM.State)
+  --(stack_ok : symState.stack = value :: symStack)
+  (symWords_ok : symState.activeWords = symActiveWords):
+  memoryExpansionCost symState mloadEVM =
+  Cₘ (value_and_activeWords_gas symActiveWords symState) - Cₘ symActiveWords := by
+  simp [memoryExpansionCost, memoryExpansionCost.μᵢ']
+  simp [Cₘ, symWords_ok]
+
+theorem X_mload_summary (symState : EVM.State)
+                         (symStack_ok : symStack.length < 1024):
+  let ss := {symState with
+    stack := offset :: symStack,
+    pc := .ofNat 0
+    gasAvailable := symGasAvailable,
+    executionEnv := {symState.executionEnv with
+                  code := ⟨#[(0x51 : UInt8)]⟩,
+                  codeOwner := symCodeOwner
+                  perm := symPerm},
+    accountMap := symAccounts,
+    activeWords := symActiveWords,
+    memory := symMemory,
+    substate := {symState.substate with
+                 accessedStorageKeys :=  symAccessedStorageKeys
+                 refundBalance := symRefund}
+    returnData := symReturnData,
+    execLength := symExecLength}
+  -- Assume we have enough gas
+  GasConstants.Gverylow < symGasAvailable.toNat - (memoryExpansionCost ss Operation.MLOAD) →
+  memoryExpansionCost ss Operation.MLOAD < UInt256.size →
+  X symGasAvailable.toNat symValidJumps ss =
+  .ok (.success {ss with
+          stack := (EvmYul.MachineState.lookupMemory ss.toMachineState offset) :: symStack,
+          pc := .ofNat 1,
+          gasAvailable := symGasAvailable - .ofNat (memoryExpansionCost ss mloadEVM) - .ofNat GasConstants.Gverylow,
+          activeWords := activeWords_comp offset symActiveWords
+          returnData := .empty,
+          execLength := symExecLength + 2} .empty) := by
+  intro ss enoughGas mec_small
+  have gavail_pos : 1 < symGasAvailable.toNat := by
+    rw [GasConstants.Gverylow] at enoughGas; omega
+  cases g_case : symGasAvailable.toNat; omega
+  rename_i g_pos
+  simp [X, C', δ]
+  have lt_fls_rw {n m : ℕ} (_ : n < m) : (m < n) = False := by
+    simp; apply Nat.ge_of_not_lt; simp; omega
+  simp [(lt_fls_rw enoughGas), α/- , (lt_fls_rw symStack_ok) -/]
+  have fls1 : (symGasAvailable.toNat < memoryExpansionCost ss (@Operation.MLOAD .EVM)) = False :=  by
+    rw [Nat.lt_sub_iff_add_lt] at enoughGas
+    aesop (add safe (by omega)) (add safe (by linarith)) (add simp [Cₘ, MachineState.M])
+  have decode_rw : ((decode ss.executionEnv.code ss.pc).getD ⟨@Operation.STOP .EVM, none⟩).1 = Operation.MLOAD := rfl
+  have gavail_rw1 : ss.gasAvailable.toNat = symGasAvailable.toNat := rfl
+  have gavail_rw2 : ss.gasAvailable = symGasAvailable := rfl
+  simp [decode_rw, gavail_rw1, gavail_rw2, fls1]
+  simp [InstructionGasGroups.Wcopy, InstructionGasGroups.Wextaccount,
+  InstructionGasGroups.Wzero, InstructionGasGroups.Wbase, InstructionGasGroups.Wverylow]
+  have fls2 : ((symGasAvailable - UInt256.ofNat (memoryExpansionCost ss Operation.MLOAD)).toNat < GasConstants.Gverylow) = False := by
+    apply eq_false_intro; rw [Nat.not_lt]
+    rw [UInt256.toNat_sub_dist, UInt256.ofNat_toNat] <;>
+    aesop (add simp [UInt256.ofNat_le, UInt256.ofNat_toNat])
+  have ss_lt2_f  (n : ℕ) : (n + 1 + 1 < 2) = False := by simp
+  simp [fls2, ss, ss_lt2_f, Nat.not_lt_of_lt symStack_ok]
+  simp [memoryExpansionCost_mload symActiveWords, value_and_activeWords_gas, ss] at fls1
+  split; aesop (add safe (by omega)) (add safe (by linarith)) (add safe (by contradiction))
+  next state n state_ok =>
+  repeat split at state_ok <;>
+  try aesop (add safe (by omega)) (add safe (by linarith)) (add safe (by contradiction))
+  cases state_ok
+  have g_pos_pos : 0 < g_pos := by omega
+  have step_rw (g : UInt256) := (EVM.step_mload_summary g_pos GasConstants.Gverylow symStack (.ofNat 0) (symGasAvailable - g) symRefund offset symActiveWords symExecLength symReturnData ⟨#[(0x51 : UInt8)]⟩ symMemory symAccessedStorageKeys symAccounts symCodeOwner symPerm g_pos_pos symState)
+  simp [EVM.step_mload, mload_instr, mloadEVM, ss] at step_rw
+  simp [step_rw, Except.instMonad, Except.bind]
+  rw [X_bad_pc] <;> aesop (add simp [GasConstants.Gverylow]) (add safe (by omega))
+
+end
+
+end MloadSummary
